code/Rubik/RowFoldChk.v
@@ -54,7 +54,7 @@ Definition fsolved (c : int) (x : pstt) : bool :=
 Notation fmcnt d :=
   (fcount forbi fpopi
      (fruns e8numi e4biti
-        fpgi fsrci fsgri fsloi fshii fsbti
+        fpgi fsrci fsrc2i ffuli fsgri fsloi fshii fsbti
         mgri mswi mloi mhii
         p1ftab frepi fsymi twsymi dnlo_data dnhi_data fllo_data flhi_data
         fstep xstep tomemb okmvv fsolved croot sroot srch forbi fpopi
